\section{Summation identities}\label{sec: summation identities}
\begin{align}
\s{b=1}{c}\s{c=1}{b} X_{c} & = \left( X_{1}\right) 
 + \left( X_{1} + X_{2} \right) + \ldots  +\left( X_{1} + X_{2} 
 + \ldots + X_{c-1} + X_{c}\right)\\
& = c X_{1} + (c-1)X_{2} + \ldots + 2 X_{c-1} + X_{c} \\
& = \s{b=1}{c}(c+1-b)X_{b}
\end{align}â€¢

\begin{align}
\s{j=1}{i-1}\s{k=1}{j-1}(j-k)X_{k} = & [0] + \left[ X_{1}\right] 
+ \left[2X_{1} + X_{2} \right] + \left[3X_{1} + 2X_{2} +X_{3}\right] 
+ \ldots  \\
& + \left[\left(i-2\right)X_{1} + \left(i-3\right)X_{2} 
+ \left(i-4\right)X_{3} + \ldots + 3X_{i-4} + 2X_{i-3} + X_{i-1}\right]  \\
= & \left(1 + 2 + 3 + \ldots +  (i-4) + (i-3) + (i-2)\right)X_{1}   \\ 
& + \left(1 + 2 + 3 + \ldots +(i-4) + (i-3) \right)X_{2}   \\ 
& + \left(1 + 2 + 3 + \ldots + (i-4) \right)X_{3} + \ldots   \\ 
& + (1 + 2 + 3)X_{i-4} + (1+2)X_{i-3} + X_{i-2}  \\
= & \s{k=1}{i-2}k X_{1} + \s{k=1}{i-3}k X_{2}  + \ldots + \s{k=1}{2}k X_{i-3} 
+ \s{k=1}{1}kX_{i-2}  \\
= & \s{j=1}{i-2}\left(\s{k=1}{i-1-j}k\right)X_{j} = 
\frac{1}{2}\s{j=1}{i-2}(i-j)(i-j-1)X_{j}
\end{align}
